tla-tree/MissingLibrary.dfy
@@ -1,6 +1,16 @@
+module MissingLibrary {
+
 function Last<T>(s:seq<T>) : T  // TODO move to library
     requires 0<|s|
 {
     s[|s|-1]
 }
 
+function {:opaque} MapRemove<K,V>(m:map<K,V>, k:K) : (m':map<K,V>)
+    ensures m'.Keys == m.Keys - {k}
+    ensures forall j :: j in m' ==> m'[j] == m[j]
+{
+    map j | j in m && j != k :: m[j]
+}
+
+} // module
